Add subsection headers, add mirror, amphichiral, reorganise definitions logically, remove commented code, add lemma on properties

project/ToroidalElementaryCellular.thy
@@ -6,13 +6,6 @@ begin
 
 section \<open>Basic definitions of Toroidal Elementary Cellular Automata\<close>
 
-(* Generate the neighbourhoods for each cell *)
-(* this is the only function that needs to change to make different topologies!*)
-fun inner_nbhds :: "state \<Rightarrow> neighbourhood list" where
-"inner_nbhds (x#y#z#[]) = (Nb x y z) # []" |
-"inner_nbhds (x#y#z#zs) = (Nb x y z) # (inner_nbhds (y#z#zs))" |
-"inner_nbhds _ = []" (* neighbourhoods aren't defined for \<le> 2 *)
-
 fun nbhds :: "state \<Rightarrow> neighbourhood list" where
 "nbhds [] = []" | (*this should never happen*)
 "nbhds (x#xs) = ((Nb (last xs) x (hd xs)) # (inner_nbhds (x#xs))) @ [Nb (last (butlast xs)) (last xs) x]"
@@ -24,8 +17,28 @@ fun update_CA :: "CA \<Rightarrow> CA" where
 fun run_t_steps :: "CA \<Rightarrow> nat \<Rightarrow> CA" where
 "run_t_steps ca n = apply_t_times update_CA ca n"
 
-definition rule110 :: CA where
-"rule110 \<equiv> CA [Zero, One, Zero] r110" 
 
-value "State (run_t_steps rule110 5)"
+subsection \<open>Important Property Definitions\<close>
+
+definition yields :: "CA \<Rightarrow> state \<Rightarrow> bool" (infixr \<open>yields\<close>  65) where
+"A yields s \<equiv> (\<exists> n. State (run_t_steps A n) = s \<and> n > 0)"
+
+definition loops :: "CA \<Rightarrow> bool" where
+"loops ca \<equiv> ca yields State ca"
+
+fun reversible :: "CA \<Rightarrow> bool" where
+"reversible (CA _ r) = (\<forall>s. (\<exists>!s0. State (update_CA (CA s0 r)) = s))"
+
+(* maybe add some infix notation for this or other things as it looks good *)
+fun garden_of_eden :: "CA \<Rightarrow> bool" where
+"garden_of_eden (CA s r) = (\<not>(\<exists> s0. State (update_CA (CA s0 r)) = s))"
+
+lemma "garden_of_eden ca \<Longrightarrow> \<not>reversible ca"
+  by (metis garden_of_eden.elims(2) reversible.simps)
+
+
+subsection \<open> Basic Rule Examples \<close>
+
+definition rule110 :: CA where
+"rule110 \<equiv> CA [Zero, One, Zero] r110"
 end
