project/CellularBase.thy
@@ -4,8 +4,9 @@ begin
 
 section \<open>Base datatypes and definitions common to all Cellular Automata\<close>
 (* Might end up having different bases between 1 and 2D*)
-
 (* perhaps typeclass them so well-formed works on all? *)
+
+subsection \<open>Basis type of all elementary 1D CA\<close>
 
 datatype cell = One | Zero
 type_synonym state = "cell list"
@@ -13,9 +14,6 @@ datatype neighbourhood = Nb cell cell cell
 type_synonym rule = "neighbourhood \<Rightarrow> cell"
 
 datatype CA = CA (State : state) (Rule : rule)
-
-definition width :: "CA \<Rightarrow> nat" where
-"width ca = length (State ca)"
 
 consts nbhds :: "state \<Rightarrow> neighbourhood list" (* This doesn't really do anything helpful yet *)
 
@@ -25,18 +23,18 @@ fun inner_nbhds :: "state \<Rightarrow> neighbourhood list" where
 "inner_nbhds (x#y#z#zs) = (Nb x y z) # (inner_nbhds (y#z#zs))" |
 "inner_nbhds _ = []" (* neighbourhoods aren't defined for \<le> 2 *)
 
-(*fun update_CA :: "CA \<Rightarrow> CA" where
-"update_CA (CA s r) = CA (map r (nbhds s)) r"*)
-
-definition null_rule :: rule where
-"null_rule _ = Zero"
-
-(*definition testCA :: CA where
-"testCA = CA [One, One, Zero] null_rule null_edge null_edge"*)
-
 fun apply_t_times :: "('a \<Rightarrow> 'a) \<Rightarrow> 'a \<Rightarrow> nat \<Rightarrow> 'a" where
 "apply_t_times f a 0 = a" |
 "apply_t_times f a (Suc n) = apply_t_times f (f a) n"
+
+
+subsection \<open>Simple properties for CA\<close>
+
+definition width :: "CA \<Rightarrow> nat" where
+"width ca = length (State ca)"
+
+(*fun update_CA :: "CA \<Rightarrow> CA" where
+"update_CA (CA s r) = CA (map r (nbhds s)) r"*)
 
 definition wellformed :: "CA \<Rightarrow> bool" where
 "wellformed ca \<equiv> (width ca \<ge> 3)"
@@ -53,6 +51,18 @@ fun garden_of_eden :: "CA \<Rightarrow> bool" where
 fun reversible :: "CA \<Rightarrow> bool" where
 "reversible (CA _ rule l r) = (\<forall>s. (\<exists>!s0. State (run_t_steps (CA s0 rule l r) 1) = s))"*)
 
+fun mirror :: "rule \<Rightarrow> rule" where
+"mirror r (Nb a b c)= r (Nb c b a)"
+
+definition amphichiral :: "rule \<Rightarrow> bool" where
+"amphichiral r \<equiv> r = (mirror r)"
+
+
+subsection \<open>Concrete base examples\<close>
+
+definition null_rule :: rule where
+"null_rule _ = Zero"
+
 fun r110 :: rule where
 "r110  (Nb One One One) = Zero"   |
 "r110  (Nb One One Zero) = One"   |
@@ -62,4 +72,5 @@ fun r110 :: rule where
 "r110  (Nb Zero One Zero) = One"  |
 "r110  (Nb Zero Zero One) = One"  |
 "r110  (Nb Zero Zero Zero) = Zero"
+
 end
